src/opt/ReorderWrite.v
@@ -34,7 +34,7 @@ Inductive sim_write (loc:Loc.t) (val:Const.t) (ord:Ordering.t) (th_src th_tgt:Lo
 .
 
 Lemma sim_write_begin
-      loc val ord
+      loc from to val released ord
       th1_src mem1_src
       th1_tgt mem1_tgt
       th2_tgt mem2_tgt
@@ -42,7 +42,7 @@ Lemma sim_write_begin
       (MEMORY1: sim_memory mem1_src mem1_tgt)
       (WF1_SRC: Local.wf th1_src mem1_src)
       (WF1_TGT: Local.wf th1_tgt mem1_tgt)
-      (STEP_TGT: Local.memory_step th1_tgt mem1_tgt (MemEvent.write loc val ord) th2_tgt mem2_tgt):
+      (STEP_TGT: Local.write_step th1_tgt mem1_tgt loc from to val released ord th2_tgt mem2_tgt):
   (<<LOCAL2: sim_write loc val ord th1_src th2_tgt>> /\
    <<MEMORY2: sim_memory mem1_src mem2_tgt>>) \/
   (exists th2_src mem2_src,
@@ -54,7 +54,7 @@ Proof.
   - left. splits; auto.
     inversion LOCAL1. apply MemInv.sem_bot_inv in PROMISE.
     destruct th1_src, th1_tgt. ss. subst.
-    inv CONFIRM.
+    inv FULFILL.
     econs; s.
     + eapply CommitFacts.write_mon; eauto.
     + reflexivity.
@@ -76,7 +76,7 @@ Proof.
       * eapply Commit.future_wf; eauto. apply WF1_SRC.
     + inversion LOCAL1. apply MemInv.sem_bot_inv in PROMISE0.
       destruct th1_src, th1_tgt. ss. subst.
-      inv CONFIRM.
+      inv FULFILL.
       econs; s.
       * eapply CommitFacts.write_mon; eauto.
       * reflexivity.
@@ -93,8 +93,8 @@ Lemma sim_write_end
       (MEMORY1: sim_memory mem1_src mem1_tgt)
       (WF1_SRC: Local.wf th1_src mem1_src)
       (WF1_TGT: Local.wf th1_tgt mem1_tgt):
-  exists th2_src mem2_src,
-    <<STEP_SRC: Local.memory_step th1_src mem1_src (MemEvent.write loc val ord) th2_src mem2_src>> /\
+  exists from to released th2_src mem2_src,
+    <<STEP_SRC: Local.write_step th1_src mem1_src loc from to val released ord th2_src mem2_src>> /\
     <<LOCAL2: sim_local th2_src th1_tgt>> /\
     <<MEMORY2: sim_memory mem2_src mem1_tgt>>.
 Proof.
@@ -115,43 +115,14 @@ Proof.
   { apply WF1_SRC. }
   { inv WF1_SRC. inv MEMORY. exploit WF; eauto. }
   i. des.
-  eexists _, _. splits; eauto.
+  eexists _, _, _, _, _. splits; eauto.
   - econs; eauto. econs 1.
-    + inv PROMISE. econs; ss.
-    + rewrite ORD2. ss.
-  - econs; ss.
-    + rewrite <- COMMIT2. eapply CommitFacts.write_min_min. eauto.
+    + inv PROMISE. econs; eauto.
+    + destruct ord; ss.
+  - econs; s.
+    + etransitivity; eauto.
+      eapply CommitFacts.write_min_min. eauto.
     + apply MemInv.sem_bot.
-Qed.
-
-Lemma sim_local_promise
-      th1_src mem1_src
-      th1_tgt mem1_tgt
-      th2_tgt mem2_tgt
-      (LOCAL1: sim_local th1_src th1_tgt)
-      (MEMORY1: sim_memory mem1_src mem1_tgt)
-      (WF1_SRC: Local.wf th1_src mem1_src)
-      (WF1_TGT: Local.wf th1_tgt mem1_tgt)
-      (STEP_TGT: Local.promise_step th1_tgt mem1_tgt th2_tgt mem2_tgt):
-  exists th2_src mem2_src,
-    <<STEP_SRC: Local.promise_step th1_src mem1_src th2_src mem2_src>> /\
-    <<LOCAL2: sim_local th2_src th2_tgt>> /\
-    <<MEMORY2: sim_memory mem2_src mem2_tgt>>.
-Proof.
-  inv LOCAL1. inv STEP_TGT.
-  exploit MemInv.promise; eauto.
-  { apply WF1_SRC. }
-  { apply WF1_TGT. }
-  i. des.
-  exploit Memory.promise_future; try apply PROMISE_SRC; eauto.
-  { apply WF1_SRC. }
-  { apply WF1_SRC. }
-  i. des.
-  eexists _, _. splits; eauto.
-  - econs; try apply PROMISE_SRC.
-    + reflexivity.
-    + eapply Commit.future_wf; [|eauto]. apply WF1_SRC.
-  - econs; s; eauto. etransitivity; eauto.
 Qed.
 
 Lemma sim_write_promise
@@ -188,22 +159,21 @@ Qed.
 
 Lemma sim_write_read
       loc1 val1 ord1
-      loc2 val2 ord2
+      loc2 ts2 val2 released2 ord2
       th1_src mem1_src
       th1_tgt mem1_tgt
-      th2_tgt mem2_tgt
+      th2_tgt
       (LOC: loc1 <> loc2)
       (ORD1: Ordering.le ord1 Ordering.relaxed)
-      (ORD2: Ordering.le ord2 Ordering.relaxed)
+      (ORD2: Ordering.le ord2 Ordering.release)
       (LOCAL1: sim_write loc1 val1 ord1 th1_src th1_tgt)
       (MEMORY1: sim_memory mem1_src mem1_tgt)
       (WF1_SRC: Local.wf th1_src mem1_src)
       (WF1_TGT: Local.wf th1_tgt mem1_tgt)
-      (STEP_TGT: Local.memory_step th1_tgt mem1_tgt (MemEvent.read loc2 val2 ord2) th2_tgt mem2_tgt):
-  exists th2_src mem2_src,
-    <<STEP_SRC: Local.memory_step th1_src mem1_src (MemEvent.read loc2 val2 ord2) th2_src mem2_src>> /\
-    <<LOCAL2: sim_write loc1 val1 ord1 th2_src th2_tgt>> /\
-    <<MEMORY2: sim_memory mem2_src mem2_tgt>>.
+      (STEP_TGT: Local.read_step th1_tgt mem1_tgt loc2 ts2 val2 released2 ord2 th2_tgt):
+  exists th2_src,
+    <<STEP_SRC: Local.read_step th1_src mem1_src loc2 ts2 val2 released2 ord2 th2_src>> /\
+    <<LOCAL2: sim_write loc1 val1 ord1 th2_src th2_tgt>>.
 Proof.
   inv LOCAL1. inv STEP_TGT.
   exploit Memory.le_get.
@@ -214,7 +184,7 @@ Proof.
   }
   intro GET1_SRC.
   exploit Memory.splits_get; try apply GET; eauto.
-  { inv MEMORY1. eauto. }
+  { apply MEMORY1. }
   intro GET2_SRC.
   exploit CommitFacts.read_min_spec; try apply GET2_SRC; eauto.
   { inv COMMIT. eapply Snapshot.readable_mon; eauto.
@@ -233,7 +203,7 @@ Proof.
   { instantiate (1 := ord1). destruct ord1; ss. }
   { apply WF1_SRC. }
   i. des.
-  eexists _, _. splits; eauto.
+  eexists _. splits; eauto.
   - econs; eauto. inv PROMISE.
     match goal with
     | [|- ?x = None] => destruct x eqn:X; auto
@@ -243,6 +213,9 @@ Proof.
   - econs; eauto. s.
     exploit CommitFacts.write_min_min; try apply COMMIT1; eauto. i.
     exploit CommitFacts.read_min_min; try apply COMMIT; eauto. i.
+    unfold CommitFacts.read_min in *.
+    destruct (Ordering.le Ordering.acquire ord2) eqn:ORD2'.
+    { destruct ord2; ss. }
     inv x0. inv x1.
     apply Snapshot.incr_writes_inv in CURRENT1.
     apply Snapshot.incr_reads_inv in CURRENT2. des.
@@ -274,7 +247,7 @@ Qed.
 
 Lemma sim_write_write
       loc1 val1 ord1
-      loc2 val2 ord2
+      loc2 from2 to2 val2 released2 ord2
       th1_src mem1_src
       th1_tgt mem1_tgt
       th2_tgt mem2_tgt
@@ -284,9 +257,9 @@ Lemma sim_write_write
       (MEMORY1: sim_memory mem1_src mem1_tgt)
       (WF1_SRC: Local.wf th1_src mem1_src)
       (WF1_TGT: Local.wf th1_tgt mem1_tgt)
-      (STEP_TGT: Local.memory_step th1_tgt mem1_tgt (MemEvent.write loc2 val2 ord2) th2_tgt mem2_tgt):
+      (STEP_TGT: Local.write_step th1_tgt mem1_tgt loc2 from2 to2 val2 released2 ord2 th2_tgt mem2_tgt):
   exists th2_src mem2_src,
-    <<STEP_SRC: Local.memory_step th1_src mem1_src (MemEvent.write loc2 val2 ord2) th2_src mem2_src>> /\
+    <<STEP_SRC: Local.write_step th1_src mem1_src loc2 from2 to2 val2 released2 ord2 th2_src mem2_src>> /\
     <<LOCAL2: sim_write loc1 val1 ord1 th2_src th2_tgt>> /\
     <<MEMORY2: sim_memory mem2_src mem2_tgt>>.
 Proof.
@@ -345,7 +318,7 @@ Proof.
   { inv WF2. exploit WF0; eauto. }
   i. des.
   eexists _, _. splits; eauto.
-  - econs 2; eauto.
+  - econs; eauto.
   - econs; eauto. s.
     exploit CommitFacts.write_min_min; try apply COMMIT1; eauto. i.
     exploit CommitFacts.write_min_min; try apply COMMIT; eauto. i.
@@ -383,27 +356,6 @@ Proof.
     + etransitivity; [apply COMMIT1|].
       etransitivity; [apply COMMIT2|]. eauto.
 Qed.
-
-Lemma sim_write_update
-      loc1 val1 ord1
-      loc2 val21 val22 ord2
-      th1_src mem1_src
-      th1_tgt mem1_tgt
-      th2_tgt mem2_tgt
-      (LOC: loc1 <> loc2)
-      (ORD1: Ordering.le ord1 Ordering.relaxed)
-      (ORD2: Ordering.le ord2 Ordering.release)
-      (LOCAL1: sim_write loc1 val1 ord1 th1_src th1_tgt)
-      (MEMORY1: sim_memory mem1_src mem1_tgt)
-      (WF1_SRC: Local.wf th1_src mem1_src)
-      (WF1_TGT: Local.wf th1_tgt mem1_tgt)
-      (STEP_TGT: Local.memory_step th1_tgt mem1_tgt (MemEvent.update loc2 val21 val22 ord2) th2_tgt mem2_tgt):
-  exists th2_src mem2_src,
-    <<STEP_SRC: Local.memory_step th1_src mem1_src (MemEvent.update loc2 val21 val22 ord2) th2_src mem2_src>> /\
-    <<LOCAL2: sim_write loc1 val1 ord1 th2_src th2_tgt>> /\
-    <<MEMORY2: sim_memory mem2_src mem2_tgt>>.
-Proof.
-Admitted.
 
 Inductive reorder l2 v2 o2: forall (i1:Instr.t), Prop :=
 | reorder_load
@@ -481,77 +433,60 @@ Proof.
     + inv LOCAL. apply MemInv.sem_bot_inv in PROMISE.
       eexists _, _, _. splits; eauto. etransitivity; eauto.
     + inv REORDER.
-      * assert (STEP: exists val th2_tgt mem2_tgt,
-                   Local.memory_step x4 mem1_tgt (MemEvent.read l1 val o1) th2_tgt mem2_tgt).
+      * assert (STEP: exists ts val released th2_tgt, Local.read_step x4 mem1_tgt l1 ts val released o1 th2_tgt).
         { admit.
           (* https://github.com/jeehoonkang/memory-model-explorer/blob/86c803103989f87a17f50e6349aa9f285104af09/formalization/src/opt/Reorder.v#L116 *)
         }
         des.
-        exploit sim_write_read; try apply LOCAL; try apply STEP; eauto. i. des.
+        exploit sim_write_read; eauto.
+        { destruct o1; ss. }
+        i. des.
         exploit sim_write_end; eauto.
-        { eapply Local.memory_step_future; eauto. }
-        { eapply Local.memory_step_future; eauto. }
+        { eapply Local.read_step_future; eauto. }
+        { eapply Local.read_step_future; eauto. }
         i. des.
         eexists _, _, _. splits.
         { econs 2; [|econs 2; [|econs 1]].
           - econs 3; eauto. econs. econs.
-          - econs 3; eauto. econs.
-            erewrite <- RegFile.eq_except_value; eauto.
+          - econs 4; s; eauto.
+            econs. erewrite <- RegFile.eq_except_value; eauto.
             + econs.
             + apply RegFile.eq_except_singleton.
         }
         inv LOCAL0. apply MemInv.sem_bot_inv in PROMISE.
         etransitivity; eauto.
         inv STEP. ss.
-      * assert (STEP: exists th2_tgt mem2_tgt,
-                   Local.memory_step x4 mem1_tgt (MemEvent.write l1 (RegFile.eval_value rs v1) o1) th2_tgt mem2_tgt).
+      * assert (STEP: exists from to released th2_tgt mem2_tgt,
+                   Local.write_step x4 mem1_tgt l1 from to (RegFile.eval_value rs v1) released o1 th2_tgt mem2_tgt).
         { admit. }
         des.
-        exploit sim_write_write; try apply LOCAL; try apply STEP; eauto. i. des.
+        exploit sim_write_write; eauto. i. des.
         exploit sim_write_end; eauto.
-        { eapply Local.memory_step_future; eauto. }
-        { eapply Local.memory_step_future; eauto. }
+        { eapply Local.write_step_future; eauto. }
+        { eapply Local.write_step_future; eauto. }
         i. des.
         eexists _, _, _. splits.
         { econs 2; [|econs 2; [|econs 1]].
-          - econs 3; eauto. econs. econs.
-          - econs 3; eauto. econs. econs.
+          - econs 4; eauto. econs. econs.
+          - econs 4; eauto. econs. econs.
         }
         inv LOCAL0. apply MemInv.sem_bot_inv in PROMISE.
         etransitivity; eauto.
         inv STEP. ss.
         rewrite PROMISE_TGT in *. eapply Memory_write_bot. eauto.
-      * assert (STEP: exists val th2_tgt mem2_tgt,
-                   Local.memory_step x4 mem1_tgt (MemEvent.update l1 val (snd (RegFile.eval_rmw rs rmw1 val)) o1) th2_tgt mem2_tgt).
-        { admit. }
-        des.
-        exploit sim_write_update; try apply LOCAL; try apply STEP0; eauto. i. des.
-        exploit sim_write_end; eauto.
-        { eapply Local.memory_step_future; eauto. }
-        { eapply Local.memory_step_future; eauto. }
-        i. des.
-        eexists _, _, _. splits.
-        { econs 2; [|econs 2; [|econs 1]].
-          - econs 3; eauto. econs. econs. apply surjective_pairing.
-          - econs 3; eauto. econs.
-            erewrite <- RegFile.eq_except_value; eauto.
-            + econs.
-            + admit. (* regfile disjoint *)
-        }
-        inv LOCAL0. apply MemInv.sem_bot_inv in PROMISE.
-        etransitivity; eauto.
-        inv STEP. ss.
-        rewrite PROMISE_TGT in *. eapply Memory_write_bot. eauto.
+      * admit. (* update *)
   - i. inv PR; ss.
     + (* begin *)
       inv STEP_TGT; inv STEP; try (inv STATE; inv INSTR); ss.
-      * exploit sim_local_promise; eauto. i. des.
+      * (* promise *)
+        exploit sim_local_promise; eauto. i. des.
         eexists _, _, _, _, _, _. splits; eauto.
         { econs. econs 1. eauto. }
         right. apply CIH. econs 1; ss.
-      * exploit sim_write_begin; eauto. i. des.
+      * (* store *)
+        exploit sim_write_begin; eauto. i. des.
         { eexists _, _, _, _, _, _. splits; try apply MEMORY2; eauto.
-          { econs. econs 3; ss.
+          { econs. econs 6; ss.
             - econs. econs.
             - apply Local.fence_relaxed. ss.
           }
@@ -559,11 +494,11 @@ Proof.
         }
         { eexists _, _, _, _, _, _. splits; try apply MEMORY2.
           { econs 2; [|econs 1].
-            econs 3; ss.
+            econs 6; ss.
             - econs. econs.
             - apply Local.fence_relaxed. ss.
           }
-          { econs. econs 1; eauto. }
+          { econs. s. econs 1. eauto. }
           right. apply CIH. econs 3; eauto.
         }
     + (* end *)
@@ -574,50 +509,64 @@ Proof.
       right. apply CIH. econs 2; ss.
     + (* intermediate *)
       inv STEP_TGT; inv STEP; try (inv STATE; inv INSTR; inversion REORDER); subst; ss.
-      * exploit sim_write_promise; eauto.
+      * (* promise *)
+        exploit sim_write_promise; eauto.
         { inv REORDER; ss. }
         i. des.
         eexists _, _, _, _, _, _. splits; eauto.
         { econs. econs 1. eauto. }
         right. apply CIH. econs 3; ss.
-      * exploit sim_write_read; try apply LOCAL; try apply STEP0; eauto. i. des.
+      * (* read *)
+        exploit sim_write_read; eauto.
+        { destruct ord; ss. }
+        i. des.
         exploit sim_write_end; eauto.
-        { eapply Local.memory_step_future; eauto. }
-        { eapply Local.memory_step_future; eauto. }
+        { eapply Local.read_step_future; eauto. }
+        { eapply Local.read_step_future; eauto. }
         i. des.
         eexists _, _, _, _, _, _. splits.
         { econs 2; [|econs 1].
           econs 3; eauto. econs. econs.
         }
-        { econs. econs 3; eauto. econs.
+        { econs. econs 4; eauto. econs.
           erewrite <- RegFile.eq_except_value; eauto.
           - econs.
           - apply RegFile.eq_except_singleton.
         }
         { eauto. }
         right. apply CIH. econs 2; eauto.
-      * exploit sim_write_write; try apply LOCAL; try apply STEP; eauto. i. des.
+      * (* write *)
+        exploit sim_write_write; eauto. i. des.
         exploit sim_write_end; eauto.
-        { eapply Local.memory_step_future; eauto. }
-        { eapply Local.memory_step_future; eauto. }
+        { eapply Local.write_step_future; eauto. }
+        { eapply Local.write_step_future; eauto. }
         i. des.
         eexists _, _, _, _, _, _. splits.
         { econs 2; [|econs 1].
-          econs 3; eauto. econs. econs.
+          econs 4; eauto. econs. econs.
         }
-        { econs. econs 3; eauto. econs. econs. }
+        { econs. econs 4; eauto. econs. econs. }
         { eauto. }
         right. apply CIH. econs 2; eauto.
-      * exploit sim_write_update; try apply LOCAL; try apply STEP0; eauto. i. des.
+      * (* update *)
+        exploit sim_write_read; eauto. i. des.
+        exploit sim_write_write; eauto.
+        { eapply Local.read_step_future; eauto. }
+        { eapply Local.read_step_future; eauto. }
+        i. des.
         exploit sim_write_end; eauto.
-        { eapply Local.memory_step_future; eauto. }
-        { eapply Local.memory_step_future; eauto. }
+        { eapply Local.write_step_future; eauto.
+          eapply Local.read_step_future; eauto.
+        }
+        { eapply Local.write_step_future; eauto.
+          eapply Local.read_step_future; eauto.
+        }
         i. des.
         eexists _, _, _, _, _, _. splits.
         { econs 2; [|econs 1].
-          econs 3; eauto. econs. econs. eauto.
+          econs 5; eauto. econs. econs. eauto.
         }
-        { econs. econs 3; eauto. econs.
+        { econs. econs 4; eauto. econs.
           erewrite <- RegFile.eq_except_value; eauto.
           - econs.
           - admit. (* regfile disjoint *)
